fill in proofs for PCUIC

erasure/theories/EWcbvEvalInd.v
@@ -24,20 +24,6 @@ Definition atomic_term (t : term) :=
   
 Lemma All_tip {A} {P : A -> Type} {a : A} : P a <~> All P [a].
 Proof. split; intros. repeat constructor; auto. now depelim X. Qed.
-  
-Fixpoint eval_depth {wfl : WcbvFlags} {Σ : global_declarations} {t1 t2 : term} (ev : eval Σ t1 t2) { struct ev } : nat.
-Proof.
-  rename eval_depth into aux.
-  destruct ev.
-  all:try match goal with
-  | [ H : eval _ _ _, H' : eval _ _ _, H'' : eval _ _ _ |- _ ] => 
-    apply aux in H; apply aux in H'; apply aux in H''; exact (S (Nat.max H (Nat.max H' H'')))
-  | [ H : eval _ _ _, H' : eval _ _ _ |- _ ] => 
-    apply aux in H; apply aux in H'; exact (S (Nat.max H H'))
-  | [ H : eval _ _ _ |- _ ] => apply aux in H; exact (S H)
-  end.
-  exact 1.
-Defined.
 
 Lemma eval_construct_size  {fl : WcbvFlags} [Σ kn c args e] : 
   forall (ev : eval Σ (mkApps (tConstruct kn c) args) e),
@@ -63,152 +49,137 @@ Qed.
 
 Section eval_mkApps_rect.
   
-Variables (wfl : WcbvFlags) (Σ : global_declarations) 
-  (P : term → term → Type).
+  Variables (wfl : WcbvFlags) (Σ : global_declarations) (P : term → term → Type).
 
   Let IH x y (ev : eval Σ x y) := 
     forall t u (ev' : eval Σ t u), eval_depth ev' <= eval_depth ev -> P t u.
 
-
-Lemma eval_mkApps_rect :
-  (∀ a t t' : term,
-	  forall ev : eval Σ a tBox, P a tBox → 
-    IH _ _ ev ->
-    eval Σ t t' → P t t' → P (tApp a t) tBox)
-  → (∀ (f0 : term) (na : BasicAst.name) (b a a' res : term),
-       forall ev : eval Σ f0 (tLambda na b),
-       P f0 (tLambda na b) → IH _ _ ev → 
-       eval Σ a a' → P a a'
-             → eval Σ (ECSubst.csubst a' 0 b) res
-               → P (ECSubst.csubst a' 0 b) res → P (tApp f0 a) res)
+  Lemma eval_mkApps_rect :
+    (∀ a t t' : term,
+	    forall ev : eval Σ a tBox, P a tBox → 
+                            IH _ _ ev ->
+                            eval Σ t t' → P t t' → P (tApp a t) tBox)
+    → (∀ (f0 : term) (na : BasicAst.name) (b a a' res : term),
+        forall ev : eval Σ f0 (tLambda na b),
+          P f0 (tLambda na b)
+          → IH _ _ ev
+          → eval Σ a a' →
+          P a a'
+          → eval Σ (ECSubst.csubst a' 0 b) res
+          → P (ECSubst.csubst a' 0 b) res → P (tApp f0 a) res)
     → (∀ (na : BasicAst.name) (b0 b0' b1 res : term),
-         eval Σ b0 b0'
-         → P b0 b0'
-           → eval Σ (ECSubst.csubst b0' 0 b1) res
-             → P (ECSubst.csubst b0' 0 b1) res → P (tLetIn na b0 b1) res)
-      → (∀ (ind : Kernames.inductive) (pars : nat) (discr : term) 
-           (c : nat) (args : list term) (brs : 
-                                              list 
-                                                (list BasicAst.name × term)) 
-           (br : list BasicAst.name × term) (res : term),
-           eval Σ discr (mkApps (tConstruct ind c) args)
-           → P discr (mkApps (tConstruct ind c) args)
-             → inductive_isprop_and_pars Σ ind = Some (false, pars)
-               → nth_error brs c = Some br
-                 → #|skipn pars args| = #|br.1|
-                   → eval Σ (iota_red pars args br) res
-                     → P (iota_red pars args br) res
-                       → P (tCase (ind, pars) discr brs) res)
-        → (∀ (ind : Kernames.inductive) (pars : nat) (discr : term) 
-             (brs : list (list BasicAst.name × term)) 
-             (n : list BasicAst.name) (f3 res : term),
-             with_prop_case
-             → eval Σ discr tBox
-               → P discr tBox
-                 → inductive_isprop_and_pars Σ ind = Some (true, pars)
-                   → brs = [(n, f3)]
-                     → eval Σ (ECSubst.substl (repeat tBox #|n|) f3)
-                         res
-                       → P (ECSubst.substl (repeat tBox #|n|) f3) res
-                         → P (tCase (ind, pars) discr brs) res)
-          → (∀ (f4 : term) (mfix : mfixpoint term) 
-               (idx : nat) (argsv : list term) 
-               (a av fn res : term),
-               forall guarded : with_guarded_fix,
-               forall ev : eval Σ f4 (mkApps (tFix mfix idx) argsv),
-               P f4 (mkApps (tFix mfix idx) argsv)
-               → IH _ _ ev
-                 → eval Σ a av
-                   → P a av
-                     → cunfold_fix mfix idx = Some (#|argsv|, fn)
-                       → eval Σ (tApp (mkApps fn argsv) av) res
-                         → P (tApp (mkApps fn argsv) av) res
-                           → P (tApp f4 a) res)
-            → (∀ (f5 : term) (mfix : mfixpoint term) 
-                 (idx : nat) (argsv : list term) 
-                 (a av : term) (narg : nat) (fn : term),
-                 forall guarded : with_guarded_fix,
-                 forall ev : eval Σ f5 (mkApps (tFix mfix idx) argsv),
-                 P f5 (mkApps (tFix mfix idx) argsv) → IH _ _ ev
-                 → eval Σ a av
-                     → P a av
-                       → cunfold_fix mfix idx = Some (narg, fn)
-                         → #|argsv| < narg
-                           → P (tApp f5 a)
-                               (tApp
-                                  (mkApps (tFix mfix idx) argsv) av))
-            → (∀ (f6 : term) (mfix : mfixpoint term) 
-                   (idx : nat) (a fn res : term) (narg : nat) 
-                   (unguarded : with_guarded_fix = false) 
-                   (ev : eval Σ f6 (tFix mfix idx)),
-                   P f6 (tFix mfix idx)
-                   → IH _ _ ev
-                   → ∀ (e0 : cunfold_fix mfix idx = Some (narg, fn)) 
-                       (e1 : eval Σ (tApp fn a) res),
-                       P (tApp fn a) res
-                       → P (tApp f6 a) res)
-              → (∀ (ip : Kernames.inductive × nat) (mfix : mfixpoint term) 
-                   (idx : nat) (args : list term) 
-                   (narg : nat) discr (fn : term) (brs : 
-                                                 list 
-                                                 (list BasicAst.name × term)) 
-                   (res : term),
-                   cunfold_cofix mfix idx = Some (narg, fn)
-                   -> eval Σ discr (mkApps (tCoFix mfix idx) args)
-                   -> P discr (mkApps (tCoFix mfix idx) args)
-                   → eval Σ (tCase ip (mkApps fn args) brs) res
-                     → P (tCase ip (mkApps fn args) brs) res
-                       → P
-                           (tCase ip discr brs)
-                           res)
-                → (∀ (p : Kernames.projection) (mfix : mfixpoint term) 
-                     (idx : nat) (args : list term) 
-                     (narg : nat) discr (fn res : term),
-                     cunfold_cofix mfix idx = Some (narg, fn)
-                     -> eval Σ discr (mkApps (tCoFix mfix idx) args)
-                     -> P discr (mkApps (tCoFix mfix idx) args)
-                     → eval Σ (tProj p (mkApps fn args)) res
-                       → P (tProj p (mkApps fn args)) res
-                         → P
-                             (tProj p discr) res)
-                  → (∀ (c : Kernames.kername) (decl : constant_body) 
-                       (body : term),
-                       declared_constant Σ c decl
-                       → ∀ res : term,
-                           cst_body decl = Some body
-                           → eval Σ body res
-                             → P body res → P (tConst c) res)
-                    → (∀ (i : inductive) (pars arg : nat) 
-                         (discr : term) (args : list term) 
-                         (res : term),
-                         eval Σ discr
-                           (mkApps (tConstruct i 0) args)
-                         → P discr (mkApps (tConstruct i 0) args)
-                           → inductive_isprop_and_pars Σ i = Some (false, pars)
-                             → eval Σ (nth (pars + arg) args tDummy) res
-                               → P (nth (pars + arg) args tDummy) res
-                                 → P (tProj (i, pars, arg) discr) res)
-                      → (∀ (i : inductive) (pars arg : nat) 
-                           (discr : term),
-                           with_prop_case
-                           → eval Σ discr tBox
-                             → P discr tBox
-                               → inductive_isprop_and_pars Σ i = Some (true, pars)
-                                 → P (tProj (i, pars, arg) discr)
-                                     tBox)
-                        → (∀ (f11 f' : term) a a' ,
-                             forall (ev : eval Σ f11 f'),
-                              P f11 f' ->
-                            IH _ _ ev
-                            → ~~
-                                 (isLambda f' || (if with_guarded_fix then isFixApp f' else isFix f')
-                                  || isBox f')
-                                 → eval Σ a a'
-                                → P a a'
-                          →  P (tApp f11 a) (tApp f' a'))
-                                  
-                          → (∀ t : term, atom t → P t t)
-                            → ∀ t t0 : term, eval Σ t t0 → P t t0.
+          eval Σ b0 b0'
+          → P b0 b0'
+          → eval Σ (ECSubst.csubst b0' 0 b1) res
+          → P (ECSubst.csubst b0' 0 b1) res →
+          P (tLetIn na b0 b1) res)
+    → (∀ (ind : Kernames.inductive) (pars : nat) (discr : term) 
+         (c : nat) (args : list term) (brs : list  (list BasicAst.name × term)) 
+         (br : list BasicAst.name × term) (res : term),
+          eval Σ discr (mkApps (tConstruct ind c) args)
+          → P discr (mkApps (tConstruct ind c) args)
+          → inductive_isprop_and_pars Σ ind = Some (false, pars)
+          → nth_error brs c = Some br
+          → #|skipn pars args| = #|br.1|
+          → eval Σ (iota_red pars args br) res
+          → P (iota_red pars args br) res
+          → P (tCase (ind, pars) discr brs) res)
+    → (∀ (ind : Kernames.inductive) (pars : nat) (discr : term) 
+         (brs : list (list BasicAst.name × term)) 
+         (n : list BasicAst.name) (f3 res : term),
+          with_prop_case
+          → eval Σ discr tBox
+          → P discr tBox
+          → inductive_isprop_and_pars Σ ind = Some (true, pars)
+          → brs = [(n, f3)]
+          → eval Σ (ECSubst.substl (repeat tBox #|n|) f3) res
+          → P (ECSubst.substl (repeat tBox #|n|) f3) res
+          → P (tCase (ind, pars) discr brs) res)
+    → (∀ (f4 : term) (mfix : mfixpoint term) 
+         (idx : nat) (argsv : list term) 
+         (a av fn res : term),
+        forall guarded : with_guarded_fix,
+        forall ev : eval Σ f4 (mkApps (tFix mfix idx) argsv),
+          P f4 (mkApps (tFix mfix idx) argsv)
+          → IH _ _ ev
+          → eval Σ a av
+          → P a av
+          → cunfold_fix mfix idx = Some (#|argsv|, fn)
+          → eval Σ (tApp (mkApps fn argsv) av) res
+          → P (tApp (mkApps fn argsv) av) res
+          → P (tApp f4 a) res)
+    → (∀ (f5 : term) (mfix : mfixpoint term) 
+         (idx : nat) (argsv : list term) 
+         (a av : term) (narg : nat) (fn : term),
+        forall guarded : with_guarded_fix,
+        forall ev : eval Σ f5 (mkApps (tFix mfix idx) argsv),
+          P f5 (mkApps (tFix mfix idx) argsv) 
+          → IH _ _ ev
+          → eval Σ a av
+          → P a av
+          → cunfold_fix mfix idx = Some (narg, fn)
+          → #|argsv| < narg
+          → P (tApp f5 a) (tApp (mkApps (tFix mfix idx) argsv) av))
+    → (∀ (f6 : term) (mfix : mfixpoint term) 
+         (idx : nat) (a fn res : term) (narg : nat) 
+         (unguarded : with_guarded_fix = false) 
+         (ev : eval Σ f6 (tFix mfix idx)),
+          P f6 (tFix mfix idx)
+          → IH _ _ ev
+          → cunfold_fix mfix idx = Some (narg, fn)
+          → eval Σ (tApp fn a) res
+          → P (tApp fn a) res
+          → P (tApp f6 a) res)
+    → (∀ (ip : Kernames.inductive × nat) (mfix : mfixpoint term) 
+         (idx : nat) (args : list term) 
+         (narg : nat) discr (fn : term) (brs : list (list BasicAst.name × term)) 
+         (res : term),
+          cunfold_cofix mfix idx = Some (narg, fn)
+          -> eval Σ discr (mkApps (tCoFix mfix idx) args)
+          -> P discr (mkApps (tCoFix mfix idx) args)
+          → eval Σ (tCase ip (mkApps fn args) brs) res
+          → P (tCase ip (mkApps fn args) brs) res
+          → P (tCase ip discr brs) res)
+    → (∀ (p : Kernames.projection) (mfix : mfixpoint term) 
+         (idx : nat) (args : list term) 
+         (narg : nat) discr (fn res : term),
+          cunfold_cofix mfix idx = Some (narg, fn)
+          -> eval Σ discr (mkApps (tCoFix mfix idx) args)
+          -> P discr (mkApps (tCoFix mfix idx) args)
+          → eval Σ (tProj p (mkApps fn args)) res
+          → P (tProj p (mkApps fn args)) res
+          → P (tProj p discr) res)
+    → (∀ (c : Kernames.kername) (decl : constant_body) (body : term),
+          declared_constant Σ c decl
+          → ∀ res : term,
+          cst_body decl = Some body
+          → eval Σ body res
+          → P body res → P (tConst c) res)
+    → (∀ (i : inductive) (pars arg : nat) 
+         (discr : term) (args : list term) 
+         (res : term),
+          eval Σ discr (mkApps (tConstruct i 0) args)
+          → P discr (mkApps (tConstruct i 0) args)
+          → inductive_isprop_and_pars Σ i = Some (false, pars)
+          → eval Σ (nth (pars + arg) args tDummy) res
+          → P (nth (pars + arg) args tDummy) res
+          → P (tProj (i, pars, arg) discr) res)
+    → (∀ (i : inductive) (pars arg : nat) (discr : term),
+          with_prop_case
+          → eval Σ discr tBox
+          → P discr tBox
+          → inductive_isprop_and_pars Σ i = Some (true, pars)
+          → P (tProj (i, pars, arg) discr) tBox)
+    → (∀ (f11 f' : term) a a' ,
+        forall (ev : eval Σ f11 f'),
+          P f11 f' ->
+          IH _ _ ev
+          → ~~ (isLambda f' || (if with_guarded_fix then isFixApp f' else isFix f') || isBox f')
+          → eval Σ a a'
+          → P a a'
+          → P (tApp f11 a) (tApp f' a'))
+    → (∀ t : term, atom t → P t t)
+    → ∀ t t0 : term, eval Σ t t0 → P t t0.
 Proof.
   intros.
   pose proof (p := @Fix_F { t : _ & { t0 : _ & eval Σ t t0 }}).
@@ -567,3 +538,4 @@ Proof.
   - unshelve eapply X12; tea.
     all:try (intros; apply and_assum; [ih|intros hp'; split => //; eapply P'Q; tea]).
 Qed.
+
