pcuic/theories/TemplateToPCUICExpanded.v
@@ -12,18 +12,21 @@ Tactic Notation "wf_inv" ident(H) simple_intropattern(p) :=
 
 Local Hint Constructors expanded : expanded.
 
-(* Lemma trans_expanded {cf : checker_flags} {Σ} {wfΣ : Template.Typing.wf Σ} T :
+Lemma trans_expanded {cf : checker_flags} {Σ} {wfΣ : Template.Typing.wf Σ} Γ T  :
   let Σ' := trans_global_env Σ in
   WfAst.wf Σ T ->
-  EtaExpand.expanded Σ T ->
-  expanded Σ' (trans Σ' T).
+  EtaExpand.expanded Σ Γ T ->
+  expanded Σ' Γ (trans Σ' T).
 Proof with eauto using expanded.
   intros Σ' wf exp. revert wf.
   induction exp; intros wf; cbn -[Σ']...
   all: try now (wf_inv wf []; eauto using expanded).
   all: try now (wf_inv wf [[]]; eauto using expanded).
-  - wf_inv wf ?. econstructor; eauto. solve_all.
-  - wf_inv wf []. eapply expanded_mkApps with (args := [_]); cbn...
+  - wf_inv wf ?. eapply expanded_tRel with (args := []). eauto. lia. econstructor.
+  - wf_inv wf [[[]]]. eapply expanded_tRel. eauto. len. solve_all.
+  - wf_inv wf [[[]]]. econstructor. solve_all.
+  - wf_inv wf []. cbn. eapply expanded_mkApps with (args := [_]); cbn... econstructor. 
+    eapply expanded_tRel with (args := []). reflexivity. lia. econstructor.
   - wf_inv wf [[[]]].
     forward IHexp; eauto.
     eapply expanded_mkApps; eauto. 2:solve_all.
@@ -36,16 +39,16 @@ Proof with eauto using expanded.
     unfold Σ'.
     erewrite trans_lookup_inductive, declared_inductive_lookup; eauto.
     econstructor; eauto. cbn. induction a1; cbn; econstructor.
-    + cbn. inversion H0; subst. eapply H3. eapply r.
+    + cbn. inversion H0; subst. rewrite map2_bias_left_length. len. eapply H3. eapply r.
     + inversion H0; subst. inversion H; subst. eapply IHa1; eauto.
     + eapply template_to_pcuic_env; eauto.
   - wf_inv wf [[]]. wf_inv w ?. eapply expanded_tFix.
-    + solve_all.
+    + solve_all. revert H0. now rewrite mapi_cst_map rev_map_spec map_map.
     + solve_all.
     + destruct args; cbn; congruence.
-    + now rewrite nth_error_map H4.
+    + now rewrite nth_error_map H5.
     + now simpl_list.
   - wf_inv wf ?. econstructor. solve_all.
   - wf_inv wf [[[]]]. eapply forall_decls_declared_constructor in H; eauto. 2: now eapply template_to_pcuic_env.
     eapply expanded_tConstruct_app. eauto. cbn. unfold trans_local. now rewrite map_length context_assumptions_map. solve_all.
-Qed. *)
+Qed. 
